src/datatype/parse/ParseDatatype.sig
@@ -4,8 +4,13 @@ sig
   datatype pretype =
     dVartype of string | dTyop of (string * pretype list) |
     dAQ of Type.hol_type
-  type datatypeAST =
-    string (* type name *) * ((string * pretype list) list)
+
+  val pretypeToType : pretype -> Type.hol_type
+
+  datatype datatypeForm =
+    WithConstructors of ((string * pretype list) list) |
+    RecordType of (string * pretype) list
+  type datatypeAST = string (* type name *) * datatypeForm
 
    val parse : Type.hol_type frag list -> datatypeAST list
 
