src/datatype/record/RecordType.sig
@@ -1,19 +1,14 @@
 signature RecordType =
 sig
- val create_term_fn 
-    : string -> Thm.thm -> ((string * Term.term) list -> Term.term)
 
-  val create_term_fn_base 
-    : bool -> string -> Thm.thm -> ((string * Term.term) list -> Term.term)
-
-  val create_term_fn_vars 
-    : string -> Thm.thm -> ((string * Term.term) list -> Term.term)
-
-  val create_record 
-    : string -> (string * Type.hol_type) list ->
+  val create_record :
+    string -> (string * Type.hol_type) list ->
       {acc_upd_thm : Thm.thm, accessor_fns : Thm.thm, cases_thm : Thm.thm,
        cons_11_thm : Thm.thm, create_fn :
          (string * Term.term) list -> Term.term, fn_upd_thm : Thm.thm list,
        type_axiom : Thm.thm, upd_acc_thm : Thm.thm, upd_canon_thm : Thm.thm,
        upd_upd_thm : Thm.thm, update_fns : Thm.thm}
+
+  val prim_define_recordtype :
+    string -> (string * Type.hol_type) list -> (TypeBase.tyinfo * string list)
 end
